x86/Asmgenproof.v
@@ -18,6 +18,31 @@ Require Import Values Memory Events Globalenvs Smallstep.
 Require Import Op Locations Mach Conventions Asm.
 Require Import Asmgen Asmgenproof0 Asmgenproof1.
 
+(** * Calling convention *)
+
+Definition cc_asmgen_mq: query li_mach -> query li_asm -> Prop :=
+  fun '(mq fb sp ra ms m1) '(State rs m2) =>
+    rs#PC = Vptr fb Ptrofs.zero /\
+    rs#RA = ra /\
+    agree ms sp rs /\
+    Mem.extends m1 m2.
+
+Definition cc_asmgen_mr: _ -> _ -> reply li_mach -> reply li_asm -> Prop :=
+  fun '(mq fb sp ra ms m1) '(State rs m2) '(ms', m1') '(State rs' m2') =>
+    rs'#PC = ra /\
+    agree ms' sp rs' /\
+    Mem.extends m1' m2'.
+
+Definition cc_asmgen: callconv li_mach li_asm :=
+  {|
+    world_def := unit;
+    match_senv w := eq;
+    match_query_def w := cc_asmgen_mq;
+    match_reply_def w := cc_asmgen_mr;
+  |}.
+
+(** * .. *)
+
 Definition match_prog (p: Mach.program) (tp: Asm.program) :=
   match_program (fun _ f tf => transf_fundef f = OK tf) eq p tp.
 
@@ -364,43 +389,60 @@ Qed.
 - Mach register values and PPC register values agree.
 *)
 
-Section WITHINITSPRA.
+Section IN_WORLD.
 
-Variables init_sp init_ra: val.
+Context (w: world cc_asmgen).
+Let sp0 := mq_sp (world_q1 w).
+Let ra0 := mq_ra (world_q1 w).
 
-Inductive match_states: Mach.state -> Asm.state -> Prop :=
+Inductive match_states: Mach.state -> Asm.mstate -> Prop :=
   | match_states_intro:
       forall s fb sp c ep ms m m' rs f tf tc
-        (STACKS: match_stack ge s)
+        (STACKS: match_stack sp0 ra0 ge s)
         (FIND: Genv.find_funct_ptr ge fb = Some (Internal f))
         (MEXT: Mem.extends m m')
         (AT: transl_code_at_pc ge (rs PC) fb f c ep tf tc)
         (AG: agree ms sp rs)
-        (AXP: ep = true -> rs#RAX = parent_sp init_sp s),
+        (AXP: ep = true -> rs#RAX = parent_sp s),
       match_states (Mach.State s fb sp c ms m)
-                   (Asm.State rs m')
+                   (Asm.State rs m', sp0, ra0)
   | match_states_call:
       forall s fb ms m m' rs
-        (STACKS: match_stack ge s)
+        (STACKS: match_stack sp0 ra0 ge s)
         (MEXT: Mem.extends m m')
-        (AG: agree ms (parent_sp init_sp s) rs)
+        (AG: agree ms (parent_sp s) rs)
         (ATPC: rs PC = Vptr fb Ptrofs.zero)
-        (ATLR: rs RA = parent_ra init_ra s),
+        (ATLR: rs RA = parent_ra s),
       match_states (Mach.Callstate s fb ms m)
-                   (Asm.State rs m')
+                   (Asm.State rs m', sp0, ra0)
   | match_states_return:
       forall s ms m m' rs
-        (STACKS: match_stack ge s)
+        (STACKS: match_stack sp0 ra0 ge s)
         (MEXT: Mem.extends m m')
-        (AG: agree ms (parent_sp init_sp s) rs)
-        (RA_VUNDEF: rs RA = Vundef)
-        (ATPC: rs PC = parent_ra init_ra s),
+        (AG: agree ms (parent_sp s) rs)
+        (ATPC: rs PC = parent_ra s),
       match_states (Mach.Returnstate s ms m)
-                   (Asm.State rs m').
+                   (Asm.State rs m', sp0, ra0).
+
+Lemma plus_step_mstep s t s':
+  plus step tge s t s' ->
+  plus mstep tge (s, sp0, ra0) t (s', sp0, ra0).
+Proof.
+  clear.
+  intros H. pattern s, t, s'. revert H.
+  apply plus_ind2.
+  - intros.
+    apply plus_one.
+    constructor; eauto.
+  - intros.
+    eapply plus_trans; eauto.
+    apply plus_one.
+    constructor; eauto.
+Qed.
 
 Lemma exec_straight_steps:
   forall s fb f rs1 i c ep tf tc m1' m2 m2' sp ms2,
-  match_stack ge s ->
+  match_stack sp0 ra0 ge s ->
   Mem.extends m2 m2' ->
   Genv.find_funct_ptr ge fb = Some (Internal f) ->
   transl_code_at_pc ge (rs1 PC) fb f (i :: c) ep tf tc ->
@@ -408,21 +450,22 @@ Lemma exec_straight_steps:
    exists rs2,
        exec_straight tge tf c rs1 m1' k rs2 m2'
     /\ agree ms2 sp rs2
-    /\ (it1_is_parent ep i = true -> rs2#RAX = parent_sp init_sp s)) ->
+    /\ (it1_is_parent ep i = true -> rs2#RAX = parent_sp s)) ->
   exists st',
-  plus step tge (State rs1 m1') E0 st' /\
+  plus mstep tge (State rs1 m1', sp0, ra0) E0 st' /\
   match_states (Mach.State s fb sp c ms2 m2) st'.
 Proof.
   intros. inversion H2. subst. monadInv H7.
   exploit H3; eauto. intros [rs2 [A [B C]]].
-  exists (State rs2 m2'); split.
+  exists (State rs2 m2', sp0, ra0); split.
+  apply plus_step_mstep.
   eapply exec_straight_exec; eauto.
   econstructor; eauto. eapply exec_straight_at; eauto.
 Qed.
 
 Lemma exec_straight_steps_goto:
   forall s fb f rs1 i c ep tf tc m1' m2 m2' sp ms2 lbl c',
-  match_stack ge s ->
+  match_stack sp0 ra0 ge s ->
   Mem.extends m2 m2' ->
   Genv.find_funct_ptr ge fb = Some (Internal f) ->
   Mach.find_label lbl f.(Mach.fn_code) = Some c' ->
@@ -434,7 +477,7 @@ Lemma exec_straight_steps_goto:
     /\ agree ms2 sp rs2
     /\ exec_instr tge tf jmp rs2 m2' = goto_label tf lbl rs2 m2') ->
   exists st',
-  plus step tge (State rs1 m1') E0 st' /\
+  plus mstep tge (State rs1 m1', sp0, ra0) E0 st' /\
   match_states (Mach.State s fb sp c' ms2 m2) st'.
 Proof.
   intros. inversion H3. subst. monadInv H9.
@@ -445,10 +488,11 @@ Proof.
   intros [ofs' [PC2 CT2]].
   exploit find_label_goto_label; eauto.
   intros [tc' [rs3 [GOTO [AT' OTH]]]].
-  exists (State rs3 m2'); split.
+  exists (State rs3 m2', sp0, ra0); split.
   eapply plus_right'.
+  apply plus_step_mstep.
   eapply exec_straight_steps_1; eauto.
-  econstructor; eauto.
+  constructor. econstructor; eauto.
   eapply find_instr_tail. eauto.
   rewrite C. eexact GOTO.
   traceEq.
@@ -474,21 +518,13 @@ Definition measure (s: Mach.state) : nat :=
 
 (** This is the simulation diagram.  We prove it by case analysis on the Mach transition. *)
 
-Hypothesis init_sp_not_vundef: init_sp <> Vundef.
-Hypothesis init_ra_not_vundef: init_ra <> Vundef.
-
-Hypothesis init_sp_type: Val.has_type init_sp Tptr.
-Hypothesis init_ra_type: Val.has_type init_ra Tptr.
-
 Theorem step_simulation:
-  forall S1 t S2, Mach.step init_sp init_ra return_address_offset ge S1 t S2 ->
+  forall S1 t S2, Mach.step return_address_offset ge S1 t S2 ->
   forall S1' (MS: match_states S1 S1'),
-  exists w, (exists t', match_events_query _ w t t') /\
-  forall t', match_events cc_extends w t t' ->
-  (exists S2', plus step tge S1' t' S2' /\ match_states S2 S2')
+  (exists S2', plus mstep tge S1' t S2' /\ match_states S2 S2')
   \/ (measure S2 < measure S1 /\ t = E0 /\ match_states S2 S1')%nat.
 Proof.
-  induction 1; intros; inv MS; try stable_step.
+  induction 1; intros; inv MS.
 
 - (* Mlabel *)
   left; eapply exec_straight_steps; eauto; intros.
@@ -523,7 +559,7 @@ Local Transparent destroyed_by_setstack.
   unfold load_stack in *.
   exploit Mem.loadv_extends. eauto. eexact H0. auto.
   intros [parent' [A B]]. rewrite (sp_val _ _ _ AG) in A.
-  exploit (lessdef_parent_sp init_sp); eauto. clear B; intros B; subst parent'.
+  exploit lessdef_parent_sp; eauto. clear B; intros B; subst parent'.
   exploit Mem.loadv_extends. eauto. eexact H1. auto.
   intros [v' [C D]].
 Opaque loadind.
@@ -604,13 +640,12 @@ Opaque loadind.
     econstructor; eauto.
   exploit return_address_offset_correct; eauto. intros; subst ra.
   left; econstructor; split.
-  apply plus_one. eapply exec_step_internal. eauto.
+  apply plus_one. constructor. eapply exec_step_internal. eauto.
   eapply functions_transl; eauto. eapply find_instr_tail; eauto.
   simpl. eauto.
   econstructor; eauto.
   econstructor; eauto.
   eapply agree_sp_def; eauto.
-  eapply agree_sp_type; eauto.
   simpl. eapply agree_exten; eauto. intros. Simplifs.
   Simplifs. rewrite <- H2. auto.
 + (* Direct call *)
@@ -619,13 +654,12 @@ Opaque loadind.
     econstructor; eauto.
   exploit return_address_offset_correct; eauto. intros; subst ra.
   left; econstructor; split.
-  apply plus_one. eapply exec_step_internal. eauto.
+  apply plus_one. constructor. eapply exec_step_internal. eauto.
   eapply functions_transl; eauto. eapply find_instr_tail; eauto.
   simpl. unfold Genv.symbol_address. rewrite symbols_preserved. rewrite H. eauto.
   econstructor; eauto.
   econstructor; eauto.
   eapply agree_sp_def; eauto.
-  eapply agree_sp_type; eauto.
   simpl. eapply agree_exten; eauto. intros. Simplifs.
   Simplifs. rewrite <- H2. auto.
 
@@ -637,8 +671,8 @@ Opaque loadind.
   rewrite (sp_val _ _ _ AG) in *. unfold load_stack in *.
   exploit Mem.loadv_extends. eauto. eexact H1. auto. simpl. intros [parent' [A B]].
   exploit Mem.loadv_extends. eauto. eexact H2. auto. simpl. intros [ra' [C D]].
-  exploit (lessdef_parent_sp init_sp); eauto. intros. subst parent'. clear B.
-  exploit (lessdef_parent_ra init_ra); eauto. intros. subst ra'. clear D.
+  exploit lessdef_parent_sp; eauto. intros. subst parent'. clear B.
+  exploit lessdef_parent_ra; eauto. intros. subst ra'. clear D.
   exploit Mem.free_parallel_extends; eauto. intros [m2' [E F]].
   destruct ros as [rf|fid]; simpl in H; monadInv H7.
 + (* Indirect call *)
@@ -649,35 +683,33 @@ Opaque loadind.
     exploit ireg_val; eauto. rewrite H7; intros LD; inv LD; auto.
   generalize (code_tail_next_int _ _ _ _ NOOV H8). intro CT1.
   left; econstructor; split.
-  eapply plus_left. eapply exec_step_internal. eauto.
+  eapply plus_left. constructor. eapply exec_step_internal. eauto.
   eapply functions_transl; eauto. eapply find_instr_tail; eauto.
   simpl. replace (chunk_of_type Tptr) with Mptr in * by (unfold Tptr, Mptr; destruct Archi.ptr64; auto).
   rewrite C. rewrite A. rewrite <- (sp_val _ _ _ AG). rewrite E. eauto.
-  apply star_one. eapply exec_step_internal.
+  apply star_one. constructor. eapply exec_step_internal.
   transitivity (Val.offset_ptr rs0#PC Ptrofs.one). auto. rewrite <- H4. simpl. eauto.
   eapply functions_transl; eauto. eapply find_instr_tail; eauto.
   simpl. eauto. traceEq.
   econstructor; eauto.
   apply agree_set_other; auto. apply agree_nextinstr. apply agree_set_other; auto.
   eapply agree_change_sp; eauto. eapply parent_sp_def; eauto.
-  eapply parent_sp_type; eauto.
   Simplifs. rewrite Pregmap.gso; auto.
   generalize (preg_of_not_SP rf). rewrite (ireg_of_eq _ _ EQ1). congruence.
 + (* Direct call *)
   generalize (code_tail_next_int _ _ _ _ NOOV H8). intro CT1.
   left; econstructor; split.
-  eapply plus_left. eapply exec_step_internal. eauto.
+  eapply plus_left. constructor. eapply exec_step_internal. eauto.
   eapply functions_transl; eauto. eapply find_instr_tail; eauto.
   simpl. replace (chunk_of_type Tptr) with Mptr in * by (unfold Tptr, Mptr; destruct Archi.ptr64; auto).
   rewrite C. rewrite A. rewrite <- (sp_val _ _ _ AG). rewrite E. eauto.
-  apply star_one. eapply exec_step_internal.
+  apply star_one. constructor. eapply exec_step_internal.
   transitivity (Val.offset_ptr rs0#PC Ptrofs.one). auto. rewrite <- H4. simpl. eauto.
   eapply functions_transl; eauto. eapply find_instr_tail; eauto.
   simpl. eauto. traceEq.
   econstructor; eauto.
   apply agree_set_other; auto. apply agree_nextinstr. apply agree_set_other; auto.
   eapply agree_change_sp; eauto. eapply parent_sp_def; eauto.
-  eapply parent_sp_type; eauto.
   rewrite Pregmap.gss. unfold Genv.symbol_address. rewrite symbols_preserved. rewrite H. auto.
 
 - (* Mbuiltin *)
@@ -686,10 +718,8 @@ Opaque loadind.
   generalize (transf_function_no_overflow _ _ H3); intro NOOV.
   exploit builtin_args_match; eauto. intros [vargs' [P Q]].
   exploit external_call_mem_extends; eauto.
-  intros (w & Hwq & Hw). exists w; split; eauto.
-  intros t' Ht'. specialize (Hw t' Ht').
-  destruct Hw as [vres' [m2' [A [B [C D]]]]].
-  left. econstructor; split. apply plus_one.
+  intros [vres' [m2' [A [B [C D]]]]].
+  left. econstructor; split. apply plus_one. constructor.
   eapply exec_step_builtin. eauto. eauto.
   eapply find_instr_tail; eauto.
   erewrite <- sp_val by eauto.
@@ -713,8 +743,8 @@ Opaque loadind.
   assert (f0 = f) by congruence. subst f0.
   inv AT. monadInv H4.
   exploit find_label_goto_label; eauto. intros [tc' [rs' [GOTO [AT2 INV]]]].
-  left; exists (State rs' m'); split.
-  apply plus_one. econstructor; eauto.
+  left; exists (State rs' m', sp0, ra0); split.
+  apply plus_one. constructor. econstructor; eauto.
   eapply functions_transl; eauto.
   eapply find_instr_tail; eauto.
   simpl; eauto.
@@ -807,7 +837,7 @@ Opaque loadind.
   intros [tc' [rs' [A [B C]]]].
   exploit ireg_val; eauto. rewrite H. intros LD; inv LD.
   left; econstructor; split.
-  apply plus_one. econstructor; eauto.
+  apply plus_one. constructor. econstructor; eauto.
   eapply find_instr_tail; eauto.
   simpl. rewrite <- H9.  unfold Mach.label in H0; unfold label; rewrite H0. eexact A.
   econstructor; eauto.
@@ -824,25 +854,23 @@ Transparent destroyed_by_jumptable.
   rewrite (sp_val _ _ _ AG) in *. unfold load_stack in *.
   replace (chunk_of_type Tptr) with Mptr in * by (unfold Tptr, Mptr; destruct Archi.ptr64; auto).
   exploit Mem.loadv_extends. eauto. eexact H0. auto. simpl. intros [parent' [A B]].
-  exploit (lessdef_parent_sp init_sp); eauto. intros. subst parent'. clear B.
+  exploit lessdef_parent_sp; eauto. intros. subst parent'. clear B.
   exploit Mem.loadv_extends. eauto. eexact H1. auto. simpl. intros [ra' [C D]].
-  exploit (lessdef_parent_ra init_ra); eauto. intros. subst ra'. clear D.
+  exploit lessdef_parent_ra; eauto. intros. subst ra'. clear D.
   exploit Mem.free_parallel_extends; eauto. intros [m2' [E F]].
   monadInv H6.
   exploit code_tail_next_int; eauto. intro CT1.
   left; econstructor; split.
-  eapply plus_left. eapply exec_step_internal. eauto.
+  eapply plus_left. constructor. eapply exec_step_internal. eauto.
   eapply functions_transl; eauto. eapply find_instr_tail; eauto.
   simpl. rewrite C. rewrite A. rewrite <- (sp_val _ _ _ AG). rewrite E. eauto.
-  apply star_one. eapply exec_step_internal.
+  apply star_one. constructor. eapply exec_step_internal.
   transitivity (Val.offset_ptr rs0#PC Ptrofs.one). auto. rewrite <- H3. simpl. eauto.
   eapply functions_transl; eauto. eapply find_instr_tail; eauto.
   simpl. eauto. traceEq.
   constructor; auto.
-  apply agree_set_other; auto.
   apply agree_set_other; auto. apply agree_nextinstr. apply agree_set_other; auto.
   eapply agree_change_sp; eauto. eapply parent_sp_def; eauto.
-  eapply parent_sp_type; eauto.
 
 - (* internal function *)
   exploit functions_translated; eauto. intros [tf [A B]]. monadInv B.
@@ -857,7 +885,7 @@ Transparent destroyed_by_jumptable.
   exploit Mem.storev_extends. eexact G. eexact H2. eauto. eauto.
   intros [m3' [P Q]].
   left; econstructor; split.
-  apply plus_one. econstructor; eauto.
+  apply plus_one. constructor. econstructor; eauto.
   simpl. rewrite Ptrofs.unsigned_zero. simpl. eauto.
   simpl. rewrite C. simpl in F, P.
   replace (chunk_of_type Tptr) with Mptr in F, P by (unfold Tptr, Mptr; destruct Archi.ptr64; auto).
@@ -873,7 +901,6 @@ Transparent destroyed_at_function_entry.
   apply agree_undef_regs with rs0; eauto.
   simpl; intros. apply Pregmap.gso; auto with asmgen. tauto.
   congruence.
-  constructor.
   intros. Simplifs. eapply agree_sp; eauto.
 
 - (* external function *)
@@ -882,105 +909,94 @@ Transparent destroyed_at_function_entry.
   exploit extcall_arguments_match; eauto.
   intros [args' [C D]].
   exploit external_call_mem_extends; eauto.
-  intros (w & Hwq & Hw). exists w; split; eauto.
-  intros t' Ht'. specialize (Hw t' Ht').
-  destruct Hw as [res' [m2' [P [Q [R S]]]]].
+  intros [res' [m2' [P [Q [R S]]]]].
   left; econstructor; split.
-  apply plus_one. eapply exec_step_external; eauto.
-  {
-    destruct STACK as (m_ & FEA & t_ & res'_ & m'_ & EC).
-    inv AG.
-    exploit EraseArgs.free_extcall_args_parallel_extends.
-    eapply Val.lessdef_refl.
-    eassumption. eauto.
-    intros (m'_0 & FEA' & EXT).
-    esplit. rewrite agree_sp. split; eauto.
-    exploit external_call_mem_extends. eexact EC. eauto. eauto.
-    admit. (* can't produce a matching trace for this other execution? would need to modify the erase-arguments condition to have the shape with a world? *)
-    (*
-    intros (vres' & m2'0 & EC' & LDres & EXT' & UNCH).
-    repeat eexists.
-    eapply external_call_symbols_preserved; eauto.
-    exact senv_preserved.
-    *)
-  }
-  { (* rs SP Tint *)
-    erewrite agree_sp by eauto.
-    eapply parent_sp_type; eauto.
-  }
-  { (* rs RA Tint *)
-    rewrite ATLR.
-    eapply parent_ra_type; eauto.
-  }
-  { (* rs SP not Vundef *)
-    erewrite agree_sp by eauto.
-    eapply parent_sp_def; eauto.
-  }
-  { (* rs RA not Vundef *)
-    rewrite ATLR.
-    eapply parent_ra_def; eauto.
-  }
+  apply plus_one. constructor. eapply exec_step_external; eauto.
   eapply external_call_symbols_preserved; eauto. apply senv_preserved. auto.
   econstructor; eauto.
   unfold loc_external_result.
-  apply agree_set_other; auto.
   apply agree_set_other; auto. apply agree_set_pair; auto.
 
 - (* return *)
   inv STACKS. simpl in *.
   right. split. omega. split. auto.
   econstructor; eauto. rewrite ATPC; eauto. congruence.
-Admitted.
+Qed.
 
-End WITHINITSPRA.
+End IN_WORLD.
 
 Lemma transf_initial_states:
-  forall st1, Mach.initial_state prog st1 ->
-  exists st2, Asm.initial_state tprog st2 /\ match_states Vnullptr Vnullptr st1 st2.
+  forall w q1 q2, match_query cc_asmgen w q1 q2 ->
+  forall st1, Mach.initial_state ge q1 st1 ->
+  exists st2, Asm.initial_state tge q2 st2 /\ match_states w st1 st2.
 Proof.
-  intros. inversion H. unfold ge0 in *.
-  econstructor; split.
-  econstructor.
-  eapply (Genv.init_mem_transf_partial TRANSF); eauto.
-  replace (Genv.symbol_address (Genv.globalenv tprog) (prog_main tprog) Ptrofs.zero)
-     with (Vptr fb Ptrofs.zero).
-  econstructor; eauto.
-  constructor.
-  apply Mem.extends_refl.
-  split. reflexivity. simpl.
-  unfold Vnullptr; destruct Archi.ptr64; congruence.
-  eapply parent_sp_type. apply Val.Vnullptr_has_type. constructor.
-  intros. rewrite Regmap.gi. auto.
-  unfold Genv.symbol_address.
-  rewrite (match_program_main TRANSF).
-  rewrite symbols_preserved.
-  unfold ge; rewrite H1. auto.
-  Unshelve. eauto.
-Qed.
+  intros w q1 q2 Hq. destruct Hq.
+  destruct q1 as [fb sp ra ms m1], q2 as [rs m2], Hq as (Hpc & Hra & Hrs & Hm).
+  intros st1 Hst1. inv Hst1.
+  exists (State rs m2, sp, rs#RA).
+  pose proof Hrs as []; subst.
+  split.
+  - constructor.
+    + rewrite genv_next_preserved.
+      admit. (* facile *)
+    + admit. (* XXX: external_pc too restrictive; no mach constraint *)
+    + destruct 1.
+      edestruct functions_translated as (tf & Htf & Hf); eauto.
+      monadInv Hf.
+      congruence.
+    + destruct Hrs.
+      congruence.
+    + admit. (* RA not Vundef *)
+  - econstructor; eauto.
+    simpl.
+    constructor; eauto.
+    admit. (* RA not Vundef *)      
+Admitted.
+
+Variable (cc_compcert_ext: callconv li_c li_asm).
+
+Lemma transf_external:
+  forall w st1 st2 q1,
+    match_states w st1 st2 ->
+    Mach.at_external ge st1 q1 ->
+    exists wA q2,
+      match_query cc_compcert_ext wA q1 q2 /\
+      Asm.at_external tge st2 q2 /\
+      forall r1 r2 st1',
+        match_reply cc_compcert_ext wA r1 r2 ->
+        Mach.after_external ge st1 r1 st1' ->
+        exists st2',
+          Asm.after_external st2 r2 st2' /\
+          match_states w st1' st2'.
+Admitted.
 
 Lemma transf_final_states:
-  forall st1 st2 r,
-  match_states Vnullptr Vnullptr st1 st2 -> Mach.final_state st1 r -> Asm.final_state st2 r.
+  forall w st1 st2 r1, match_states w st1 st2 -> Mach.final_state st1 r1 ->
+  exists r2, match_reply cc_asmgen w r1 r2 /\ Asm.final_state tge st2 r2.
 Proof.
-  intros. inv H0. inv H. constructor. auto.
-  assert (r0 = AX).
-  { unfold loc_result in H1; destruct Archi.ptr64; compute in H1; congruence. }
-  subst r0.
-  generalize (preg_val _ _ _ AX AG). rewrite H2. intros LD; inv LD. auto.
-Qed.
+  intros [[] [fb sp ra ms m1] [rs m2] (Hpc & Hra & Hrs & Hm)].
+  intros. inv H0. inv H. simpl in *.
+  eexists. split; constructor.
+  - simpl.
+    inv STACKS.
+    split; eauto.
+  - admit. (* XXX need to remember init_ra is external *)
+  - inv STACKS.
+    pose proof AG as [].
+    eauto.
+Admitted.
 
 Theorem transf_program_correct:
-  forward_simulation cc_extends (Mach.semantics return_address_offset prog) (Asm.semantics tprog).
+  forward_simulation cc_compcert_ext cc_asmgen
+    (Mach.semantics return_address_offset prog)
+    (Asm.semantics tprog).
 Proof.
   eapply forward_simulation_star with (measure := measure).
   apply senv_preserved.
   eexact transf_initial_states.
+  eexact transf_external.
   eexact transf_final_states.
   intros. apply step_simulation; auto.
-  unfold Vnullptr; destruct Archi.ptr64; congruence.
-  unfold Vnullptr; destruct Archi.ptr64; congruence.
-  apply Val.Vnullptr_has_type.
-  apply Val.Vnullptr_has_type. 
 Qed.
 
 End PRESERVATION.
